\documentclass{article}
\usepackage{CTEX}
\usepackage{graphicx}
\usepackage{threeparttable}
\usepackage{float}
\usepackage{longtable}
\usepackage{ listings} 
\usepackage{eqnarray}
\usepackage{amsmath}

 \title{信号与信息处理}
% \author{姜贵平}
\begin{document}
 \maketitle
 \begin{flushright}
 姓名：姜贵平\\学号：SA17011142
 \end{flushright}
 \section{second-layer}
 \begin{align}
\frac{\partial E}{\partial w_{kj}^{(2)}}&=\frac{\partial E}{\partial {y_k}}*\frac{\partial {y_k}}{\partial w_{kj}^{(2)}}\\
&=-\frac{1}{y_k}*f'(z_k)*h(\sum\limits_{i=0}^Dw_{ji}^{(1)}*x_i)
 \end{align}


 \section{first-layer}
  \begin{align}
 \frac{\partial E}{\partial w_{ji}^{(1)}}&=\frac{\partial E}{\partial {y_k}}*\frac{\partial {y_k}}{\partial w_{ji}^{(1)}}\\
 &=-\frac{1}{y_k}*f'(z_k)*w_{kj}^{(2)}*h'(\sum\limits_{i=0}^Dw_{ji}^{(1)}*x_i)*x_i
\end{align}
  其中：
 \begin{center}
 	$z_k=\sum\limits_{j=0}^M* w_{kj}^{(2)}*h(\sum\limits_{i=0}^Dw_{ji}^{(1)}*x_i)$\\
 	$f'(x_i)=\frac{exp(x_i)*\sum\limits_{i=1}^K exp(x_i)-exp^2(x_i)}{(\sum\limits_{i=1}^K exp(x_i)^2}$\\
 	$h(x)=tanh(x)=\frac{e^{x}-e^{-x}}{e^{x}+e^{-x}}$\\
 	$h'(x)=\frac{4}{(e^{x}+e^{-x})^2}$
  \end{center}
\end{document}

